theories/Algorithmic/Subtyping/Definitions.v
@@ -1,0 +1,39 @@
+From Mcltt Require Import Base.
+From Mcltt.Core Require Import System.Definitions NbE.
+From Mcltt Require Export Syntax.
+Import Syntax_Notations.
+
+Reserved Notation "Γ ⊢a A ⊆ A'" (in custom judg at level 80, Γ custom exp, A custom exp, A' custom exp).
+Reserved Notation "⊢anf A ⊆ A'" (in custom judg at level 80, A custom nf, A' custom nf).
+
+Definition not_univ_pi (A : nf) : Prop :=
+  match A with
+  | nf_typ _ | nf_pi _ _ => False
+  | _ => True
+  end.
+
+Inductive alg_subtyping_nf : nf -> nf -> Prop :=
+| asnf_refl : forall M N,
+    not_univ_pi M ->
+    M = N ->
+    {{ ⊢anf M ⊆ N }}
+| asnf_univ : forall i j,
+    i <= j ->
+    {{ ⊢anf Type@i ⊆ Type@j }}
+| asnf_pi : forall A B A' B',
+    A = A' ->
+    {{ ⊢anf B ⊆ B' }} ->
+    {{ ⊢anf Π A B ⊆ Π A' B' }}
+where "⊢anf M ⊆ N" := (alg_subtyping_nf M N) (in custom judg) : type_scope.
+
+
+Inductive alg_subtyping : ctx -> typ -> typ -> Prop :=
+| alg_subtyp_run : forall Γ M N A B,
+    nbe_ty Γ M A ->
+    nbe_ty Γ N B ->
+    {{ ⊢anf A ⊆ B }} ->
+    {{ Γ ⊢a M ⊆ N }}
+where "Γ ⊢a M ⊆ N" := (alg_subtyping Γ M N) (in custom judg) : type_scope.
+
+#[export]
+  Hint Constructors alg_subtyping_nf alg_subtyping: mcltt.
