theories/Algorithmic/Subtyping/Lemmas.v
@@ -1,0 +1,128 @@
+From Mcltt Require Import Base LibTactics.
+From Mcltt.Core Require Import System Evaluation Readback NbE CoreTypeInversions Presup CtxSub SystemOpt.
+From Mcltt.Core.Completeness Require Import Consequences.Rules.
+From Mcltt Require Import Completeness Soundness.
+From Mcltt.Algorithmic Require Import Subtyping.Definitions.
+Import Syntax_Notations.
+
+#[local]
+  Ltac apply_subtyping :=
+  repeat match goal with
+    | H : {{ ~?Γ ⊢ ~?A : ~?M }},
+        H1 : {{ ~?Γ ⊢ ~?M ⊆ ~?N }} |- _ =>
+        assert {{ Γ ⊢ A : N }} by mauto; clear H
+    end.
+
+Lemma alg_subtyping_nf_sound : forall M N,
+    {{ ⊢anf M ⊆ N }} ->
+    forall Γ i,
+      {{ Γ ⊢ M : Type@i }} ->
+      {{ Γ ⊢ N : Type@i }} ->
+      {{ Γ ⊢ M ⊆ N }}.
+Proof.
+  induction 1; intros; subst; simpl in *.
+  - econstructor. mauto.
+  - assert (i < j \/ i = j) as H2 by lia.
+    destruct H2; mauto 3.
+  - on_all_hyp: fun H => (apply wf_pi_inversion in H; destruct H as [? ?]).
+    destruct_all.
+    gen_presups.
+    repeat match goal with
+           | H : {{ ~?Γ ⊢ ~?M ⊆ ~?N }}, H1: {{ ⊢ ~?Γ , ~_ }} |- _ =>
+               pose proof (wf_subtyp_univ_weaken _ _ _ _ H H1);
+               fail_if_dup
+           end.
+    apply_subtyping.
+    deepexec IHalg_subtyping_nf ltac:(fun H => pose proof H).
+    mauto 3.
+Qed.
+
+Lemma alg_subtyping_nf_trans : forall M1 M0 M2,
+    {{ ⊢anf M0 ⊆ M1 }} ->
+    {{ ⊢anf M1 ⊆ M2 }} ->
+    {{ ⊢anf M0 ⊆ M2 }}.
+Proof.
+  intro M1; induction M1; intros ? ? H1 H2;
+    dependent destruction H1;
+    dependent destruction H2;
+    simpl in *;
+    try contradiction;
+    mauto.
+  apply asnf_univ. lia.
+Qed.
+
+Lemma alg_subtyping_nf_refl : forall M,
+    {{ ⊢anf M ⊆ M }}.
+Proof.
+  intro M; induction M;
+    solve [constructor; simpl; trivial].
+Qed.
+
+#[local]
+ Hint Resolve alg_subtyping_nf_trans alg_subtyping_nf_refl : mcltt.
+
+Lemma alg_subtyping_trans : forall Γ M0 M1 M2,
+    {{ Γ ⊢a M0 ⊆ M1 }} ->
+    {{ Γ ⊢a M1 ⊆ M2 }} ->
+    {{ Γ ⊢a M0 ⊆ M2 }}.
+Proof.
+  intros. progressive_inversion.
+  functional_nbe_rewrite_clear.
+  mauto.
+Qed.
+
+#[local]
+ Hint Resolve alg_subtyping_trans : mcltt.
+
+
+Lemma alg_subtyping_complete : forall Γ M N,
+    {{ Γ ⊢ M ⊆ N }} ->
+    {{ Γ ⊢a M ⊆ N }}.
+Proof.
+  induction 1; mauto.
+  - apply completeness in H.
+    destruct H as [W [? ?]].
+    econstructor; mauto.
+  - assert {{ Γ ⊢ Type@i : Type@(S i) }} by mauto.
+    assert {{ Γ ⊢ Type@j : Type@(S j) }} by mauto.
+    on_all_hyp: fun H => apply soundness in H.
+    destruct_all.
+    econstructor; mauto 2.
+    progressive_inversion.
+    mauto.
+  - assert {{ Γ ⊢ Π A B : Type@i }} as HΠ1 by mauto.
+    assert {{ Γ ⊢ Π A' B' : Type@i }} as HΠ2 by mauto.
+    assert {{ ⊢ Γ , A ≈ Γ , A' }} by mauto.
+    eapply ctxeq_nbe_eq in H5; [ |eassumption].
+    match goal with
+    | H : _ |- _ => apply completeness in H
+    end.
+    apply soundness in HΠ1.
+    apply soundness in HΠ2.
+    destruct_all.
+    econstructor; mauto 2.
+    progressive_inversion.
+    simpl in *.
+    functional_initial_env_rewrite_clear.
+    simplify_evals.
+    functional_read_rewrite_clear.
+    eapply asnf_pi; trivial.
+Qed.
+
+Lemma alg_subtyping_sound : forall Γ M N i,
+    {{ Γ ⊢a M ⊆ N }} ->
+    {{ Γ ⊢ M : Type@i }} ->
+    {{ Γ ⊢ N : Type@i }} ->
+    {{ Γ ⊢ M ⊆ N }}.
+Proof.
+  intros. destruct H.
+  on_all_hyp: fun H => apply soundness in H.
+  destruct_all.
+  on_all_hyp: fun H => apply nbe_type_to_nbe_ty in H.
+  functional_nbe_rewrite_clear.
+  gen_presups.
+  eapply alg_subtyping_nf_sound in H3; try eassumption.
+  etransitivity; [mauto |].
+  etransitivity; [eassumption |].
+  mauto.
+Qed.
